src/Examples/Interval/Example_Interval_Global_Declaration.thy
@@ -26,7 +26,7 @@ definition inc_decl_eqs ::
   "pp \<times> unit \<Rightarrow> (pp \<times> unit, unit, (ivl exec_dg_st, ivl exec_dg_st) dg_state) strategy_tree"
 where
   "inc_decl_eqs =
-     dg_gen_of (unit_dg_spec_st_for inc_gs (ivl_tf_st_for inc_gs) (ivl_enter_st_for inc_gs))
+     dg_gen_of (ownership_split_dg_spec_st_for inc_gs (ivl_tf_st_for inc_gs) (ivl_enter_st_for inc_gs))
        inc_g bot cinit_ivl_st (restrict_global_resolved_q cinit_ivl_st)"
 
 lemma inc_decl_terminates:
